VeriPB/Tactic/Sat/Tests/Differential.lean
@@ -116,5 +116,6 @@ end VeriPB.Tests.Differential
 open VeriPB.Tests.Differential in
 #eval show IO Unit from do
   let d := "VeriPB/Tactic/Sat/Tests/data/"
-  for n in ["php21", "red_subproof", "red_swap", "red_const", "red_neglit", "dom_basic"] do
+  for n in ["php21", "red_subproof", "red_swap", "red_const", "red_neglit", "dom_basic",
+      "weaken_cases"] do
     runOne n (d ++ n ++ ".opb") (d ++ n ++ "_kernel.pbp")
